ironfleet/src/Dafny/Distributed/Impl/RSL/LearnerState.i.dfy
@@ -184,6 +184,7 @@ predicate LearnerState_CommonPostconditions(learner:CLearnerState, learner':CLea
 }
 
 predicate LearnerState_Process2b__Preconditions(learner:CLearnerState, executor:ExecutorState, packet:CPacket)
+  reads executor.app
 {
   && LearnerState_CommonPreconditions(learner)
   && ExecutorState_CommonPreconditions(executor)
@@ -192,6 +193,7 @@ predicate LearnerState_Process2b__Preconditions(learner:CLearnerState, executor:
 }
 
 predicate LearnerState_Process2b__Postconditions(learner:CLearnerState, executor:ExecutorState, packet:CPacket, learner':CLearnerState)
+  reads executor.app
 {
   && LearnerState_Process2b__Preconditions(learner, executor, packet)
   && LearnerState_CommonPostconditions(learner, learner')
